OneShotLeader relevant files

OneShotLeader.fst
@@ -4,9 +4,7 @@ module M = FStar.Map
 
 module S = FStar.Set
 
-module L = FStar.List.Tot
-
-open L
+module L = ListQ
 
 type msg = 
   | Vote: Node.t -> Node.t -> msg
@@ -32,30 +30,48 @@ val axm_quorum_intersection: q1: list Node.t -> q2: list Node.t
   -> Lemma (requires is_quorum q1 && is_quorum q2)
            (ensures (exists n. {:pattern (L.mem n q1); (L.mem n q2)} 
                       L.mem n q1 /\ L.mem n q2))
-           [SMTPat (is_quorum q1); SMTPat (is_quorum q2)]
+           [SMTPat (is_quorum q1); 
+            SMTPat (is_quorum q2)]
 let axm_quorum_intersection q1 q2 = admit()
 
 (*
  * Quorum monotonicity axiom. This cannot be proven just from quorum intersection since the lemma only goes one way.
  *)
 val axm_quorum_monotonic: q1:list Node.t -> q2:list Node.t
-  -> n:Node.t
   -> Lemma(requires (is_quorum q1) 
-            /\ (L.mem n q1 ==> L.mem n q2))
+            /\ (forall x. (*{:pattern (L.mem n q1); (L.mem n q2)}*)
+                  L.mem x q1 ==> L.mem x q2))
           (ensures is_quorum q2)
-          [SMTPat [(L.mem n q1);(L.mem n q2)]]
+          [SMTPat (is_quorum q1);
+           SMTPat (is_quorum q2)]
 let axm_quorum_monotonic q1 q2 = admit()
+
+val foo_thm: q1:list Node.t -> q2:list Node.t
+  -> Lemma(requires (is_quorum q1) 
+            /\ (forall x. (*{:pattern (L.mem n q1); (L.mem n q2)}*)
+                  L.mem x q1 ==> L.mem x q2))
+          (ensures is_quorum q2)
+let foo_thm q1 q2 = 
+  let _ = axm_quorum_monotonic q1 q2 in
+  ()
 
 let is_safe {leader} = 
   forall n1 n2. {:pattern (M.sel leader n1);(M.sel leader n2)} 
       M.sel leader n1 = None \/ M.sel leader n2 = None 
                 \/ M.sel leader n1 = M.sel leader n2
 
-let inductive_inv {leader;msgs;votes} =
-  forall n. {:pattern (Leader n)}
+let inv2 {msgs;votes} (n:Node.t) =
     L.mem (Leader n) msgs ==> is_quorum (M.sel votes n)
 
-let inv = inductive_inv
+let inv3 ({leader;msgs}) (n1:Node.t) (n2:Node.t) =
+  (M.sel leader n1 = Some n2) ==> L.mem (Leader n2) msgs
+
+let inv4 ({votes;msgs}) (n1:Node.t) (n2:Node.t) = 
+  L.mem n2 (M.sel votes n1)  ==> L.mem (Vote n2 n1) msgs
+
+let inv5 ({msgs}) (n1:Node.t) (n2:Node.t) (n3:Node.t) = 
+  L.mem (Vote n1 n2) msgs /\ L.mem (Vote n1 n3) msgs  
+        ==> n2 = n3
 
 #set-options "--query_stats --split_queries always"
 #set-options "--z3rlimit 1000"
@@ -68,9 +84,9 @@ let init_state = {leader = M.const None;
                   votes = M.const [];
                   msgs = []}
 
-val init_state_safe: unit -> 
-  Lemma (is_safe init_state /\ inv init_state)
-let init_state_safe () = ()
+val init_state_safe: (n:Node.t) ->
+  Lemma (is_safe init_state /\ inv2 init_state n)
+let init_state_safe n = ()
 
 
 (*
@@ -84,43 +100,64 @@ let cast_vote n s =
   else
     s
 
-val cast_vote_safe: n:Node.t -> s:state ->
-    Lemma(requires is_safe s /\ inv s)
+val cast_vote_safe: n:Node.t -> s:state 
+    -> n2:Node.t -> n3:Node.t -> n4:Node.t
+    -> n5:Node.t -> n6:Node.t -> n7:Node.t
+    -> n8:Node.t -> n9:Node.t -> 
+    Lemma(requires is_safe s /\ inv2 s n2 /\ inv3 s n3 n4
+                    /\ inv4 s n5 n6 /\ inv5 s n7 n8 n9)
          (ensures is_safe (cast_vote n s) 
-               /\ inv (cast_vote n s))
-let cast_vote_safe n s = ()
+               /\ inv2 (cast_vote n s) n2
+               /\ inv3 (cast_vote n s) n3 n4
+               /\ inv4 (cast_vote n s) n5 n6 
+               /\ inv5 (cast_vote n s) n7 n8 n9)
+let cast_vote_safe n s n2 n3 n4 n5 n6 n7 n8 n9 = ()
 
 (* recv_vote *)
-(* L.mem x (M.sel s.votes n) *)
 
-val recv_vote: s:state -> s':state{forall n x.  L.mem x (M.sel s.votes n) 
-            ==> L.mem x (M.sel s'.votes n)}
+val recv_vote: s:state -> s':state{
+       (forall n x.  L.mem x (M.sel s.votes n) 
+            ==> L.mem x (M.sel s'.votes n)) 
+    /\ (forall n. L.mem (Leader n) s'.msgs ==> L.mem (Leader n) s.msgs)}
 let recv_vote s = 
   let is_my_vote m = match m with
-    | Vote frm to -> to = self
+    | Vote frm to -> (to = self) && not(L.mem frm (M.sel s.votes self))
     | _ -> false in
-  let (my_votes,rest) = L.partition is_my_vote s.msgs in
-  match my_votes with
-    | (Vote frm _)::other -> 
-      let votes' = M.upd s.votes self ([frm]@(M.sel s.votes self)) in
-      let msgs' = other@rest in
-      {s with votes=votes'; msgs=msgs'}
+  let my_vote = L.find is_my_vote s.msgs in
+  match my_vote with
+    | Some (Vote frm _) -> 
+      let votes' = M.upd s.votes self 
+            (L.concat [frm] (M.sel s.votes self)) in
+      {s with votes=votes'}
     | _ -> s
+(*val recv_vote_monotonic_msgs: s:state -> n:Node.t
+  -> Lemma(L.mem (Leader n) s.msgs 
+            <==> L.mem (Leader n) (recv_vote s).msgs)
+            [SMTPat (L.mem (Leader n) s.msgs)]
+let recv_vote_monotonic_msgs s n = ()*)
 
-let inv2 {leader;msgs;votes} (n:Node.t) =
-    L.mem (Leader n) msgs ==> is_quorum (M.sel votes n)
-
-val recv_vote_monotonic: s:state -> n:Node.t
-  -> Lemma(forall x. L.mem x (M.sel s.votes n) 
-            ==> L.mem x (M.sel (recv_vote s).votes n))
-            [SMTPat (is_quorum (M.sel s.votes n))]
-let recv_vote_monotonic s n = ()
-
-val recv_vote_safe: s:state -> n:Node.t ->
-    Lemma(requires is_safe s /\ inv2 s n)
+val recv_vote_safe: s:state -> n1:Node.t ->
+    n2:Node.t -> n3:Node.t -> 
+    Lemma(requires is_safe s /\ inv2 s n1 /\ inv3 s n2 n3)
          (ensures is_safe (recv_vote s) 
-                /\ inv2 (recv_vote s) n)
-let recv_vote_safe s n = ()
+                /\ inv2 (recv_vote s) n1
+                /\ inv3 (recv_vote s) n2 n3)
+let recv_vote_safe s n1 n2 n3 = 
+  (*let s' = recv_vote s in
+  let _ = assert (L.mem (Leader n) s'.msgs ==> L.mem (Leader n) s.msgs) in
+  let _ = assert (L.mem (Leader n) s.msgs ==> 
+                    is_quorum (M.sel s.votes n)) in
+  let _ = assert(forall x. L.mem x (M.sel s.votes n) 
+                  ==> L.mem x (M.sel s'.votes n)) in
+  let _ = assert((is_quorum (M.sel s.votes n) /\ 
+                    (forall x. L.mem x (M.sel s.votes n) 
+                        ==> L.mem x (M.sel s'.votes n)))
+                  ==> is_quorum (M.sel s'.votes n)) in*)
+  ()
+
+(*
+ * Declare Leader
+ *)
 
 val declare_leader: state -> state
 let declare_leader s = 
@@ -129,11 +166,13 @@ let declare_leader s =
     {s with msgs = (Leader self)::s.msgs}
   else s
 
-val declare_leader_safe: s:state ->
-    Lemma(requires is_safe s /\ inv s)
+val declare_leader_safe: s:state -> n1:Node.t ->
+   n2:Node.t -> n3:Node.t ->
+    Lemma(requires is_safe s /\ inv2 s n1 /\ inv3 s n2 n3)
          (ensures is_safe (declare_leader s) 
-                /\ inv (declare_leader s))
-let declare_leader_safe s = ()
+                /\ inv2 (declare_leader s) n1
+                /\ inv3 (declare_leader s) n2 n3)
+let declare_leader_safe s n1 n2 n3 = ()
 
 
 val register_leader: state -> state
@@ -144,9 +183,12 @@ let register_leader s =
       {s with leader = M.upd s.leader self (Some n)}
   | _ -> s
 
-val register_leader_safe: s:state ->
-    Lemma(requires is_safe s)
-         (ensures is_safe (register_leader s))
-let register_leader_safe s = ()
+val register_leader_safe: s:state -> n1:Node.t ->
+    n2:Node.t -> n3:Node.t ->
+    Lemma(requires is_safe s /\ inv2 s n1 /\ inv3 s n2 n3)
+         (ensures is_safe (register_leader s)
+                  /\ inv2 (register_leader s) n1
+                  /\ inv3 (register_leader s) n2 n3)
+let register_leader_safe s n1 n2 n3 = ()
 
-
+let t = true
