ListQ.fst
@@ -1,0 +1,52 @@
+module ListQ
+
+module L = FStar.List.Tot
+
+type t a = list a
+
+let mem = L.mem
+
+val concat: #a:eqtype -> l1:list a -> l2:list a 
+  ->l:(list a){forall x. mem x l <==> mem x l1 \/ mem x l2}
+let rec concat #a l1 l2 = match l1 with
+  | [] -> l2 
+  | x::xs -> x::(concat xs l2)
+
+let (@) = concat
+
+val rev: #a:eqtype -> l1:list a 
+  -> l:list a{forall x. mem x l <==> mem x l1}
+let rec rev l1 = match l1 with
+  | [] -> []
+  | x::xs -> (rev xs)@[x]
+  
+
+val filter: #a:eqtype -> f:(a -> bool) -> l1:list a
+    -> l:list a{forall x. mem x l <==> mem x l1 /\ f x}
+let rec filter #a f l1 = match l1 with
+  | [] -> []
+  | x::xs -> if f x then x::(filter f xs)
+             else filter f xs
+
+val partition: #a:eqtype -> f:(a -> bool) -> l:list a
+    -> p:(list a * list a){let (l1,l2) = p in 
+        forall x. (*{:pattern (mem x l1); (mem x l2); (mem x l)}*)
+          mem x l <==> mem x l1 \/ mem x l2}
+let rec partition #a f l = match l with
+  | [] -> ([], [])
+  | x::xs -> let (s1,s2) = partition f xs in
+      if f x then ((x::s1),s2) else (s1,x::s2)
+
+val partition_mem_l1: #a:eqtype -> f:(a -> bool) -> l:list a
+    ->x:a 
+    ->Lemma(let (l1,l2) = partition f l in 
+              (mem x l1 ==> mem x l) /\ (mem x l2 ==> mem x l))
+let rec partition_mem_l1 #a f l x = ()
+
+val find: #a:eqtype -> f:(a -> bool) -> l:list a 
+      -> v:option a{match v with 
+          | Some x -> mem x l /\ f x
+          | None -> forall x. mem x l ==> not (f x)}
+let rec find #a f l = match l with
+  | [] -> None
+  | x::xs -> if f x then Some x else find f xs
