Node.fsti
@@ -1,0 +1,7 @@
+module Node
+
+val t : eqtype
+
+
+
+
